Code/Interpretation/OrderInterpretation.v
@@ -1,0 +1,389 @@
+Require Import Prelude.Funext.
+Require Import Prelude.CompatibleRelation.
+Require Import Syntax.Signature.
+Require Import Coq.Program.Equality.
+
+Definition TODO {A : Type} : A.
+Admitted.
+
+Section OrderInterpretation.
+  Context {B : Type}
+          (semB : B -> Type)
+          `{forall (b : B), CompatRel (semB b)}
+          `{forall (b : B), isCompatRel (semB b)}.
+
+  Fixpoint sem_Ty
+           (A : Ty B)
+    : Type
+    := match A with
+       | Base b => semB b
+       | A1 ⟶ A2 => sem_Ty A1 -> sem_Ty A2
+       end.
+
+  Global Instance sem_Ty_CompatRel
+         (A : Ty B)
+    : CompatRel (sem_Ty A).
+  Proof.
+    induction A ; apply _.
+  Defined.
+
+  Global Instance sem_Ty_isCompatRel
+         (A : Ty B)
+    : isCompatRel (sem_Ty A).
+  Proof.
+    induction A ; apply _.
+  Qed.
+    
+  Fixpoint sem_Con
+           (C : Con B)
+    : Type
+    := match C with
+       | ∙ => unit
+       | A ,, C => sem_Ty A * sem_Con C
+       end.
+
+  Global Instance sem_Con_CompatRel
+         (C : Con B)
+    : CompatRel (sem_Con C).
+  Proof.
+    induction C ; apply _.
+  Defined.
+
+  Global Instance sem_Con_isCompatRel
+         (C : Con B)
+    : isCompatRel (sem_Con C).
+  Proof.
+    induction C ; apply _.
+  Qed.
+
+  Fixpoint sem_Var
+           {C : Con B}
+           {A : Ty B}
+           (v : Var C A)
+    : sem_Con C -> sem_Ty A
+    := match v with
+       | Vz => fst
+       | Vs v => fun x => sem_Var v (snd x)
+       end.
+
+  Global Instance sem_Var_strictMonotone
+         {C : Con B}
+         {A : Ty B}
+         (v : Var C A)
+    : strictMonotone (sem_Var v).
+  Proof.
+    induction v ; apply _.
+  Qed.
+
+  Global Instance sem_Var_weakMonotone
+         {C : Con B}
+         {A : Ty B}
+         (v : Var C A)
+    : weakMonotone (sem_Var v).
+  Proof.
+    induction v ; apply _.
+  Qed.
+
+  Context {F : Type}
+          {ar : F -> Ty B}
+          (semF : forall (f : F), sem_Ty (ar f)).
+
+  Definition sem_Tm
+             {C : Con B}
+             {A : Ty B}
+             (t : Tm ar C A)
+    : sem_Con C -> sem_Ty A.
+  Proof.
+    induction t as [ ? ? f | ? ? ? v | ? ? ? ? f IHf | ? ? ? ? f IHf t IHt ].
+    - exact (fun _ => semF f).
+    - exact (sem_Var v).
+    - exact (fun x y => IHf semF (y , x)).
+    - apply TODO.
+  Defined.
+End OrderInterpretation.
+
+Global Instance sem_Tm_weakMonotone
+       {B : Type}
+       (semB : B -> Type)
+       `{forall (b : B), CompatRel (semB b)}
+       `{forall (b : B), isCompatRel (semB b)}
+       {F : Type}
+       {ar : F -> Ty B}
+       (semF : forall (f : F), sem_Ty semB (ar f))
+       {C : Con B}
+       {A : Ty B}
+       (t : Tm ar C A)
+  : weakMonotone (sem_Tm semB semF t).
+Proof.
+  induction t as [ ? ? f | ? ? ? v | ? ? ? ? f IHf | ? ? ? ? f IHf t IHt ].
+  - cbn.
+    apply _.
+  - apply _.
+  - unshelve esplit.
+    intros x y p z.
+    apply (@map_ge _ _ _ _ _ (IHf semF)).
+    split.
+    + apply ge_refl.
+    + exact p.
+  - (* unshelve esplit.
+    intros x y p ; simpl.
+    refine (ge_trans _ _).
+    + apply (@map_ge _ _ _ _ _(IHf semF) x y).
+      exact p.
+    + pose (@map_ge _ _ _ _ _(IHf semF)).
+      cbn in g.
+     *)
+    apply TODO.
+Qed.
+
+Definition sem_Wk
+           {B : Type}
+           (semB : B -> Type)
+           {C1 C2 : Con B}
+           (w : Wk C1 C2)
+  : sem_Con semB C1 -> sem_Con semB C2.
+Proof.
+  induction w as [ | ? ? ? w IHw | ? ? ? w IHw ].
+  - exact (fun _ => tt).
+  - exact (fun x => (fst x , IHw (snd x))).
+  - exact (fun x => IHw (snd x)).
+Defined.
+
+Global Instance sem_Wk_weakMonotone
+       {B : Type}
+       (semB : B -> Type)
+       `{forall (b : B), CompatRel (semB b)}
+       `{forall (b : B), isCompatRel (semB b)}
+       {C1 C2 : Con B}
+       (w : Wk C1 C2)
+  : weakMonotone (sem_Wk semB w).
+Proof.
+  induction w ; apply _.
+Qed.
+
+Global Instance sem_Wk_strictMonotone
+       {B : Type}
+       (semB : B -> Type)
+       `{forall (b : B), CompatRel (semB b)}
+       `{forall (b : B), isCompatRel (semB b)}
+       {C1 C2 : Con B}
+       (w : Wk C1 C2)
+  : strictMonotone (sem_Wk semB w).
+Proof.
+  induction w.
+  - simpl.
+    unshelve esplit.
+    simpl.
+    contradiction.
+  - apply _.
+  - apply _.
+Qed.
+
+Proposition sem_idWk
+            {B : Type}
+            (semB : B -> Type)
+            {C : Con B}
+            (x : sem_Con semB C)
+  : sem_Wk semB (idWk C) x = x.
+Proof.
+  induction C as [ | A C IHC ].
+  - destruct x.
+    reflexivity.
+  - destruct x ; simpl.
+    rewrite IHC.
+    reflexivity.
+Qed.
+
+Proposition sem_wkVar
+            {B : Type}
+            (semB : B -> Type)
+            {F : Type}
+            {ar : F -> Ty B}
+            (semF : forall (f : F), sem_Ty semB (ar f))
+            {C1 C2 : Con B}
+            (w : Wk C1 C2)
+            {A : Ty B}
+            (v : Var C2 A)
+            (x : sem_Con semB C1)
+  : sem_Tm semB semF (TmVar (wkVar v w)) x
+    =
+    sem_Tm semB semF (TmVar v) (sem_Wk semB w x).
+Proof.
+  induction w as [ | ? ? ? w IHw | ? ? ? w IHw ].
+  - cbn.
+    destruct x.
+    reflexivity.
+  - destruct x as [x1 x2].
+    dependent induction v.
+    + cbn.
+      reflexivity.
+    + simpl.
+      apply IHw.
+  - exact (IHw v (snd x)).
+Qed.
+
+Proposition sem_keepWk
+            {B : Type}
+            (semB : B -> Type)
+            {F : Type}
+            {ar : F -> Ty B}
+            (semF : forall (f : F), sem_Ty semB (ar f))
+            {C1 C2 : Con B}
+            (w : Wk C1 C2)
+            {A1 A2 : Ty B}
+            (t : Tm ar (A1 ,, C2) A2)
+            (x : sem_Con semB C1)
+            (y : sem_Ty semB A1)
+  : sem_Tm semB semF (wkTm t (Keep A1 w)) (y , x)
+    =
+    sem_Tm semB semF t (y , sem_Wk semB w x).
+Proof.
+  dependent induction t.
+  - reflexivity.
+  - dependent induction v.
+    + reflexivity.
+    + simpl.
+      exact (sem_wkVar semB semF w v x).
+  - simpl.
+    apply funext.
+    intro a.
+    simpl.
+    apply IHt ; auto.
+  - (*simpl.
+    rewrite IHt2 ; auto.
+    rewrite IHt1 ; auto.
+     *)
+    apply TODO.
+Qed.
+
+Proposition sem_dropIdWk
+            {B : Type}
+            (semB : B -> Type)
+            {F : Type}
+            {ar : F -> Ty B}
+            (semF : forall (f : F), sem_Ty semB (ar f))
+            {C : Con B}
+            {A1 A2 : Ty B}
+            (t : Tm ar C A1)
+            (x : sem_Con semB C)
+            (y : sem_Ty semB A2)
+  : sem_Tm semB semF (wkTm t (Drop A2 (idWk C))) (y , x)
+    =
+    sem_Tm semB semF t x.
+Proof.
+  induction t.
+  - reflexivity.
+  - simpl.
+    induction v.
+    + reflexivity.
+    + simpl.
+      rewrite IHv.
+      reflexivity.
+  - simpl.
+    apply funext.
+    intro z.
+    rewrite (sem_keepWk semB semF (Drop A2 (idWk C))).
+    do 2 f_equal.
+    exact (sem_idWk semB x).
+  - (*simpl.
+    rewrite IHt1, IHt2.
+    reflexivity.*)
+    apply TODO.
+Qed.
+
+Definition sem_Sub
+           {B : Type}
+           (semB : B -> Type)
+           {F : Type}
+           {ar : F -> Ty B}
+           (semF : forall (f : F), sem_Ty semB (ar f))
+           {C1 C2 : Con B}
+           (s : Sub ar C1 C2)
+  : sem_Con semB C1 -> sem_Con semB C2.
+Proof.
+  induction s as [ | ? ? ? ? s IHs t ].
+  - exact (fun _ => tt).
+  - exact (fun x => (sem_Tm semB semF t x , IHs semF x)).
+Defined.
+
+Global Instance sem_Sub_weakMonotone
+       {B : Type}
+       (semB : B -> Type)
+       `{forall (b : B), CompatRel (semB b)}
+       `{forall (b : B), isCompatRel (semB b)}
+       {F : Type}
+       {ar : F -> Ty B}
+       (semF : forall (f : F), sem_Ty semB (ar f))
+       {C1 C2 : Con B}
+       (s : Sub ar C1 C2)
+  : weakMonotone (sem_Sub semB semF s).
+Proof.
+  induction s ; apply _.
+Qed.
+
+Proposition sem_dropSub
+            {B : Type}
+            (semB : B -> Type)
+            {F : Type}
+            {ar : F -> Ty B}
+            (semF : forall (f : F), sem_Ty semB (ar f))
+            {C1 C2 : Con B}
+            (s : Sub ar C1 C2)
+            {A : Ty B}
+            (y : sem_Ty semB A)
+            (x : sem_Con semB C1)
+  : sem_Sub semB semF (dropSub s) (y , x)
+    =
+    sem_Sub semB semF s x.
+Proof.
+  induction s.
+  - reflexivity.
+  - simpl.
+    rewrite IHs.
+    rewrite sem_dropIdWk.
+    reflexivity.
+Qed.
+
+Proposition sub_Lemma
+            {B : Type}
+            (semB : B -> Type)
+            {F : Type}
+            {ar : F -> Ty B}
+            (semF : forall (f : F), sem_Ty semB (ar f))
+            {C1 C2 : Con B}
+            (s : Sub ar C1 C2)
+            {A : Ty B}
+            (t : Tm ar C2 A)
+            (x : sem_Con semB C1)
+  : sem_Tm semB semF (subTm t s) x
+    =
+    sem_Tm semB semF t (sem_Sub semB semF s x).
+Proof.
+  revert s x.
+  revert C1.
+  induction t ; intros C1 s x.
+  - reflexivity.
+  - induction v.
+    + dependent induction s.
+      reflexivity.
+    + dependent induction s.
+      exact (IHv s).
+  - simpl.
+    apply funext.
+    intro y.
+    specialize (IHt semF _ (keepSub s) (y , x)).
+    etransitivity.
+    { 
+      apply IHt.
+    }
+    simpl.
+    do 2 f_equal.
+    rewrite sem_dropSub.
+    reflexivity.
+  - (*simpl.
+    rewrite IHt1.
+    rewrite IHt2.
+    reflexivity.
+     *)
+    apply TODO.
+Qed.
