Code/Prelude/CompatibleRelation.v
@@ -1,0 +1,412 @@
+Require Import Lia.
+
+Declare Scope compat.
+Open Scope compat.
+
+Class CompatRel (X : Type) :=
+  {
+    gt : X -> X -> Prop ;
+    ge : X -> X -> Prop
+  }.
+
+Arguments gt {_} {_} _ _.
+Arguments ge {_} {_} _ _.
+
+Notation "x > y" := (gt x y) : compat.
+Notation "x >= y" := (ge x y) : compat.
+
+Class isCompatRel (X : Type) `{CompatRel X} :=
+  {
+    gt_trans : forall {x y z : X},
+      x > y -> y > z -> x > z ;
+    ge_trans : forall {x y z : X},
+      x >= y -> y >= z -> x >= z ;
+    ge_refl : forall (x : X),
+      x >= x ;
+    compat : forall {x y : X},
+      x > y -> x >= y ;
+    ge_gt : forall {x y z : X},
+      x >= y -> y > z -> x > z ;
+    gt_ge : forall {x y z : X},
+      x > y -> y >= z -> x > z
+  }.
+
+Proposition eq_gt
+            {X : Type}
+            `{isCompatRel X}
+            {x y z : X}
+            (p : x = y)
+            (q : y > z)
+  : x > z.
+Proof.
+  induction p.
+  exact q.
+Qed.
+
+Proposition gt_eq
+            {X : Type}
+            `{isCompatRel X}
+            {x y z : X}
+            (p : x > y)
+            (q : y = z)
+  : x > z.
+Proof.
+  induction q.
+  exact p.
+Qed.
+
+Proposition eq_ge
+            {X : Type}
+            `{isCompatRel X}
+            {x y z : X}
+            (p : x = y)
+            (q : y >= z)
+  : x >= z.
+Proof.
+  induction p.
+  exact q.
+Qed.
+
+Proposition ge_eq
+            {X : Type}
+            `{isCompatRel X}
+            {x y z : X}
+            (p : x >= y)
+            (q : y = z)
+  : x >= z.
+Proof.
+  induction q.
+  exact p.
+Qed.
+
+Proposition eq_to_ge
+            {X : Type}
+            `{isCompatRel X}
+            {x y : X}
+            (p : x = y)
+  : x >= y.
+Proof.
+  induction p.
+  apply ge_refl.
+Qed.
+
+Global Instance unit_CompatRel : CompatRel unit
+  := {| gt := fun _ _ => False ;
+        ge := fun _ _ => True |}.
+
+Global Instance unit_isCompatRel : isCompatRel unit.
+Proof.
+  unshelve esplit ; cbn ; auto.
+Qed.
+
+Global Instance prod_CompatRel
+       (X Y : Type)
+       `{CompatRel X}
+       `{CompatRel Y}
+  : CompatRel (X * Y)
+  := {| gt := fun x y => (fst x > fst y) /\ (snd x > snd y) ;
+        ge := fun x y => (fst x >= fst y) /\ (snd x >= snd y) |}.
+
+Global Instance prod_isCompatRel
+       (X Y : Type)
+       `{isCompatRel X}
+       `{isCompatRel Y}
+  : isCompatRel (X * Y).
+Proof.
+  unshelve esplit ; cbn.
+  - intros x y z p q ; split.
+    + refine (gt_trans _ _).
+      * apply p.
+      * apply q.
+    + refine (gt_trans _ _).
+      * apply p.
+      * apply q.
+  - intros x y z p q ; split.
+    + refine (ge_trans _ _).
+      * apply p.
+      * apply q.
+    + refine (ge_trans _ _).
+      * apply p.
+      * apply q.
+  - intros x ; split ; apply ge_refl.
+  - intros x y p ; split ; apply compat ; apply p.
+  - intros x y z p q.
+    split.
+    + refine (ge_gt _ _).
+      * apply p.
+      * apply q.
+    + refine (ge_gt _ _).
+      * apply p.
+      * apply q.
+  - intros x y z p q.
+    split.
+    + refine (gt_ge _ _).
+      * apply p.
+      * apply q.
+    + refine (gt_ge _ _).
+      * apply p.
+      * apply q.
+Qed.
+
+Global Instance depprod_CompatRel
+       {X : Type}
+       (Y : X -> Type)
+       `{forall (x : X), CompatRel (Y x)}
+  : CompatRel (forall (x : X), Y x)
+  := {| gt := fun f g => forall (x : X), f x > g x ;
+        ge := fun f g => forall (x : X), f x >= g x |}.
+
+Global Instance depprod_isCompatRel
+       {X : Type}
+       (Y : X -> Type)
+       `{forall (x : X), CompatRel (Y x)}
+       `{forall (x : X), isCompatRel (Y x)}
+  : isCompatRel (forall (x : X), Y x).
+Proof.
+  unshelve esplit ; cbn.
+  - intros f g h p q x.
+    exact (gt_trans (p x) (q x)).
+  - intros f g h p q x.
+    exact (ge_trans (p x) (q x)).
+  - intros f x.
+    exact (ge_refl (f x)).
+  - intros f g p x.
+    exact (compat (p x)).
+  - intros f g h p q x.
+    exact (ge_gt (p x) (q x)).
+  - intros f g h p q x.
+    exact (gt_ge (p x) (q x)).
+Qed.
+
+Global Instance fun_CompatRel
+       (X Y : Type)
+       `{CompatRel Y}
+  : CompatRel (X -> Y)
+  := _.
+
+Global Instance fun_isCompatRel
+       (X Y : Type)
+       `{isCompatRel Y}
+  : isCompatRel (X -> Y)
+  := _.
+
+Fixpoint power
+         (X : Type)
+         (n : nat)
+  : Type
+  := match n with
+     | 0 => unit
+     | S n => X * power X n
+     end.
+
+Notation "X ^ n" := (power X n) : compat.
+
+Global Instance power_CompatRel
+       (X : Type)
+       (n : nat)
+       `{CompatRel X}
+  : CompatRel (X ^ n).
+Proof.
+  induction n as [ | n IHn ] ; cbn.
+  - apply _.
+  - apply _.
+Defined.
+
+Global Instance power_isCompatRel
+       (X : Type)
+       (n : nat)
+       `{isCompatRel X}
+  : isCompatRel (X ^ n).
+Proof.
+  induction n as [ | n IHn ] ; cbn.
+  - apply _.
+  - apply _.
+Qed.
+
+Global Instance nat_CompatRel
+  : CompatRel nat
+  := {| gt := fun n m => n > m ;
+        ge := fun n m => n >= m |}%nat.
+
+Global Instance nat_isCompatRel
+  : isCompatRel nat.
+Proof.
+  unshelve esplit ; cbn ; intros ; lia.
+Qed.
+
+Class strictMonotone {X Y : Type} `{CompatRel X} `{CompatRel Y} (f : X -> Y) :=
+  {
+    map_gt : forall (x y : X),
+      x > y -> f x > f y
+  }.
+
+Class weakMonotone {X Y : Type} `{CompatRel X} `{CompatRel Y} (f : X -> Y) :=
+  {
+    map_ge : forall (x y : X),
+      x >= y -> f x >= f y
+  }.
+
+Global Instance const_weakMonotone
+       (X Y : Type)
+       `{CompatRel X}
+       `{isCompatRel Y}
+       (y : Y)
+  : weakMonotone (fun (_ : X) => y).
+Proof.
+  unshelve esplit.
+  intros.
+  apply ge_refl.
+Qed.
+
+Definition id {X : Type} (x : X) := x.
+Arguments id {_} _/.
+
+
+Global Instance id_strictMonotone (X : Type) `{CompatRel X}
+  : strictMonotone id.
+Proof.
+  unshelve esplit.
+  intros x y p.
+  exact p.
+Qed.
+
+Global Instance id_weakMonotone (X : Type) `{CompatRel X}
+  : weakMonotone id.
+Proof.
+  unshelve esplit.
+  intros x y p.
+  exact p.
+Qed.
+
+Definition comp
+           {X Y Z : Type}
+           (g : Y -> Z)
+           (f : X -> Y)
+           (x : X)
+  : Z
+  := g(f x).
+
+Notation "g 'o' f" := (comp g f) (at level 40, left associativity).
+Arguments comp {_ _ _} _ _ _/.
+
+Global Instance comp_strictMonotone
+       {X Y Z : Type}
+       `{HX : CompatRel X}
+       `{HY : CompatRel Y}
+       `{HZ : CompatRel Z}
+       (f : X -> Y)
+       (g : Y -> Z)
+       `{@strictMonotone _ _ HX HY f}
+       `{@strictMonotone _ _ HY HZ g}
+  : strictMonotone (g o f).
+Proof.
+  unshelve esplit.
+  intros x y p ; cbn.
+  do 2 apply map_gt.
+  assumption.
+Qed.
+
+Global Instance comp_weakMonotone
+       {X Y Z : Type}
+       `{HX : CompatRel X}
+       `{HY : CompatRel Y}
+       `{HZ : CompatRel Z}
+       (f : X -> Y)
+       (g : Y -> Z)
+       `{@weakMonotone _ _ HX HY f}
+       `{@weakMonotone _ _ HY HZ g}
+  : weakMonotone (g o f).
+Proof.
+  unshelve esplit.
+  intros x y p ; cbn.
+  do 2 apply map_ge.
+  assumption.
+Qed.
+
+Global Instance fst_strictMonotone
+       {X Y : Type}
+       `{HX : CompatRel X}
+       `{HY : CompatRel Y}
+  : strictMonotone (@fst X Y).
+Proof.
+  unshelve esplit.
+  intros x y p.
+  apply p.
+Qed.
+
+Global Instance fst_weakMonotone
+       {X Y : Type}
+       `{HX : CompatRel X}
+       `{HY : CompatRel Y}
+  : weakMonotone (@fst X Y).
+Proof.
+  unshelve esplit.
+  intros x y p.
+  apply p.
+Qed.
+
+Global Instance snd_strictMonotone
+       {X Y : Type}
+       `{HX : CompatRel X}
+       `{HY : CompatRel Y}
+  : strictMonotone (@snd X Y).
+Proof.
+  unshelve esplit.
+  intros x y p.
+  apply p.
+Qed.
+
+Global Instance snd_weakMonotone
+       {X Y : Type}
+       `{HX : CompatRel X}
+       `{HY : CompatRel Y}
+  : weakMonotone (@snd X Y).
+Proof.
+  unshelve esplit.
+  intros x y p.
+  apply p.
+Qed.
+
+Global Instance pair_weakMonotone
+       {X Y Z : Type}
+       `{HX : CompatRel X}
+       `{HY : CompatRel Y}
+       `{HZ : CompatRel Z}
+       (f : X -> Y)
+       (g : X -> Z)
+       `{@weakMonotone _ _ HX HY f}
+       `{@weakMonotone _ _ HX HZ g}
+  : weakMonotone (fun x => (f x , g x)).
+Proof.
+  unshelve esplit.
+  intros x y p.
+  split.
+  - simpl.
+    apply map_ge.
+    assumption.
+  - simpl.
+    apply map_ge.
+    assumption.
+Qed.
+
+Global Instance pair_strictMonotone
+       {X Y Z : Type}
+       `{HX : CompatRel X}
+       `{HY : CompatRel Y}
+       `{HZ : CompatRel Z}
+       (f : X -> Y)
+       (g : X -> Z)
+       `{@strictMonotone _ _ HX HY f}
+       `{@strictMonotone _ _ HX HZ g}
+  : strictMonotone (fun x => (f x , g x)).
+Proof.
+  unshelve esplit.
+  intros x y p.
+  split.
+  - simpl.
+    apply map_gt.
+    assumption.
+  - simpl.
+    apply map_gt.
+    assumption.
+Qed.
