Code/Prelude/Funext.v
@@ -1,0 +1,13 @@
+Require Import Coq.Logic.FunctionalExtensionality.
+
+(** Abbreviation for functional extensionality *)
+Definition funext
+           {A : Type}
+           {B : A -> Type}
+           {f g : forall (a : A), B a}
+           (p : forall (a : A), f a = g a)
+  : f = g.
+Proof.
+  apply functional_extensionality_dep.
+  exact p.
+Qed.
