Code/Syntax/Signature.v
@@ -3,3 +3,4 @@ Require Export Syntax.Signature.Contexts.
 Require Export Syntax.Signature.Terms.
 Require Export Syntax.Signature.TermWeakenings.
 Require Export Syntax.Signature.TermSubstitutions.
+Require Export Syntax.Signature.RewritingSystem.
