Code/Syntax/Signature/RewritingSystem.v
@@ -1,0 +1,45 @@
+Require Import Syntax.Signature.Types.
+Require Import Syntax.Signature.Contexts.
+Require Import Syntax.Signature.Terms.
+Require Import Syntax.Signature.TermWeakenings.
+Require Import Syntax.Signature.TermSubstitutions.
+
+Inductive Rew
+          {B : Type}
+          {F : Type}
+          {ar : F -> Ty B}
+          {R : Type}
+          {Rcon : R -> Con B}
+          {Rtar : R -> Ty B}
+  : forall (lhs rhs : forall (r : R), Tm ar (Rcon r) (Rtar r))
+           {C : Con B}
+           {A : Ty B},
+    Tm ar C A -> Tm ar C A -> Type
+  :=
+| Trans : forall {lhs rhs : forall (r : R), Tm ar (Rcon r) (Rtar r)}
+                 {C : Con B}
+                 {A : Ty B}
+                 {t1 t2 t3 : Tm ar C A},
+    Rew lhs rhs t1 t2 -> Rew lhs rhs t2 t3 -> Rew lhs rhs t1 t3
+| Rew_App_l : forall {lhs rhs : forall (r : R), Tm ar (Rcon r) (Rtar r)}
+                     {C : Con B}
+                     {A B : Ty B}
+                     {f1 f2 : Tm ar C (A ⟶ B)}
+                     (x : Tm ar C A),
+    Rew lhs rhs f1 f2 -> Rew lhs rhs (f1 · x) (f2 · x)
+| Rew_App_r : forall {lhs rhs : forall (r : R), Tm ar (Rcon r) (Rtar r)}
+                     {C : Con B}
+                     {A B : Ty B}
+                     (f : Tm ar C (A ⟶ B))
+                     {x1 x2 : Tm ar C A},
+    Rew lhs rhs x1 x2 -> Rew lhs rhs (f · x1) (f · x2)
+| Rew_Lam : forall {lhs rhs : forall (r : R), Tm ar (Rcon r) (Rtar r)}
+                   {C : Con B}
+                   {A B : Ty B}
+                   {f1 f2 : Tm ar (A ,, C) B},
+    Rew lhs rhs f1 f2 -> Rew lhs rhs (λ f1) (λ f2)
+| BaseRew : forall {lhs rhs : forall (r : R), Tm ar (Rcon r) (Rtar r)}
+                   {C : Con B}
+                   (r : R)
+                   (s : Sub ar C (Rcon r)),
+    Rew lhs rhs (subTm (lhs r) s) (subTm (rhs r) s).
